coqc_sofar.sh
@@ -1,0 +1,118 @@
+#!/bin/bash
+
+COMMON=(
+       #Common
+       Errors.v
+       AST.v 
+       Values.v
+       Linking.v
+       MemPerm.v
+       Memdata.v
+       Assoc.v
+       StackADT.v
+       Memtype.v
+       Memory.v
+       Globalenvs.v
+       Events.v
+       StackInj.v
+       Smallstep.v
+       Behaviors.v
+       Switch.v
+       Determinism.v
+       Unityping.v
+       Separation.v
+       )
+
+BACKEND=(
+	#Backend
+	./backend/Cminor.v
+	./x86/Op.v
+	./backend/CminorSel.v
+	./x86/SelectOp.v
+	./backend/SplitLong.v
+	./x86/SelectLong.v
+	./backend/SelectDiv.v
+	./x86/Machregs.v
+	./backend/Selection.v
+	./x86/SelectOpproof.v
+	./backend/SplitLongproof.v
+	./x86/SelectLongproof.v
+	./backend/SelectDivproof.v
+	./backend/Selectionproof.v
+	./backend/Registers.v
+	./backend/RTL.v
+	./backend/RTLgen.v
+	./backend/RTLgenspec.v
+	./backend/RTLgenproof.v
+	#Tailcall
+	#Inlining
+	./backend/Renumber.v
+	./backend/Renumberproof.v
+	./backend/Locations.v
+	./x86/Conventions1.v
+	./backend/Conventions.v
+	./backend/RTLtyping.v
+	./backend/Kildall.v
+	./backend/Liveness.v
+	./backend/ValueDomain.v
+	./x86/ValueAOp.v
+	./backend/ValueAnalysis.v
+	./x86/ConstpropOp.v
+	./backend/Constprop.v
+	./x86/ConstpropOpproof.v
+	./backend/Constpropproof.v
+	./backend/CSEdomain.v
+	./x86/CombineOp.v
+	./backend/CSE.v
+	./x86/CombineOpproof.v
+	./backend/CSEproof.v
+	./backend/NeedDomain.v
+	./x86/NeedOp.v
+	./backend/Deadcode.v
+	./backend/Deadcodeproof.v
+	./backend/Inlining.v
+	./backend/Inliningspec.v
+	)
+
+FRONTEND=(
+        #Frontend
+        Ctypes.v
+        Cop.v
+        Csyntax.v
+        Csem.v
+        Ctyping.v
+        Cstrategy.v
+        Cexec.v
+        #Cexecimpl.v
+        Initializers.v
+        Initializersproof.v
+        Clight.v
+        ClightBigstep.v
+        SimplExpr.v
+        SimplExprspec.v
+        SimplExprproof.v
+        SimplLocals.v
+        SimplLocalsproof.v
+        Csharpminor.v
+        Cshmgen.v
+        Cshmgenproof.v
+        Cminorgen.v
+        Cminorgenproof.v
+        )
+       
+COQC="coqc -R flocq compcert.flocq -R lib compcert.lib -R x86_32 compcert.x86_32 -R x86 compcert.x86 -R Common compcert.common -R cfrontend compcert.cfrontend -R driver compcert.driver -R backend compcert.backend"
+
+for i in "${COMMON[@]}"; do
+    echo "$i"
+    $COQC "./common/$i"
+done
+
+for i in "${BACKEND[@]}"; do
+    echo "$i"
+    $COQC "$i"
+done
+
+for i in "${FRONTEND[@]}"; do
+    echo "$i"
+    $COQC "./cfrontend/$i"
+done
